src/opt/Simulation.v
@@ -1,27 +1,16 @@
 Require Import sflib.
 
+Require Import Basic.
 Require Import Event.
-Require Import Memory.
+Require Import Thread.
 Require Import Configuration.
-Require Import Program.
 
 Set Implicit Arguments.
-
-Inductive tausteps: forall (src:Configuration.t) (src':Configuration.t), Prop :=
-| tausteps_nil
-    src:
-    tausteps src src
-| tausteps_cons
-    src src' src''
-    (STEP: Configuration.step src None src')
-    (STEPS: tausteps src' src''):
-    tausteps src src''
-.
 
 (* TODO: liveness *)
 Module Simulation.
   Section Simulation.
-    Variable (prog_src prog_tgt:Program.syntax).
+    Variable (prog_src prog_tgt:Configuration.syntax).
     Variable (sim: forall (src tgt:Configuration.t), Prop).
 
     Definition INIT: Prop := sim (Configuration.init prog_src) (Configuration.init prog_tgt).
@@ -47,32 +36,24 @@ Module Simulation.
     Definition FEASIBLE: Prop :=
       forall src tgt
         (SIM: sim src tgt)
-        (FEASIBLE: InceptionSet.Empty tgt.(Configuration.memory).(Memory.inceptions)),
+        (CONFIRM: ~ Messages.declared tgt.(Configuration.messages)),
         Configuration.feasible src.
 
     Definition BASE_STEP: Prop :=
-      forall src0 tgt0 tgt2
+      forall src0 tgt0 reading tgt2
         (SIM: sim src0 tgt0)
-        (STEP: Configuration.base_step tgt0 tgt2),
+        (STEP: Configuration.base_step tgt0 reading tgt2)
+        (VALIDATION:
+           forall (READING: reading),
+           exists src0' tgt0',
+             <<SRC: Configuration.internal_steps src0 src0'>> /\
+             <<TGT: Configuration.internal_steps tgt0 tgt0'>> /\
+             <<CONFIRM: ~ Messages.declared tgt0'.(Configuration.messages)>> /\
+             <<SIM: sim src0' tgt0'>>),
       exists src1 src2,
         <<INTERNAL: Configuration.internal_steps src0 src1>> /\
         <<STEP: Configuration.internal_step src1 src2>> /\
         <<SIM: sim src2 tgt2>>.
-
-    Definition INCEPTION_STEP: Prop :=
-      forall src0 src1
-        c0_tgt th0_tgt m0_tgt
-        c1_tgt th1_tgt m1_tgt
-        inception
-        (STEPS_TGT: Configuration.internal_steps (Configuration.mk c0_tgt th0_tgt m0_tgt) (Configuration.mk c1_tgt th1_tgt m1_tgt))
-        (INCEPTION: Memory.inception m0_tgt m1_tgt inception)
-        (SIM0: sim src0 (Configuration.mk c0_tgt th0_tgt m0_tgt))
-        (STEPS_SRC: Configuration.internal_steps src0 src1)
-        (SIM1: sim src1 (Configuration.mk c1_tgt th1_tgt m1_tgt)),
-      exists src1 src2,
-        <<INTERNAL: Configuration.internal_steps src0 src1>> /\
-        <<STEP: Configuration.internal_step src1 src2>> /\
-        <<SIM: sim src2 (Configuration.mk c0_tgt th0_tgt (Memory.mk m0_tgt.(Memory.buffers) (InceptionSet.add inception m0_tgt.(Memory.inceptions))))>>.
 
     Definition EXTERNAL_STEP: Prop :=
       forall src0 tgt0 e tgt2
@@ -83,7 +64,7 @@ Module Simulation.
         <<STEP: Configuration.external_step src1 e src2>> /\
         <<SIM: sim src2 tgt2>>.
 
-    Lemma internal_step (B:BASE_STEP) (I:INCEPTION_STEP):
+    Lemma internal_step (B:BASE_STEP):
       forall src0 tgt0 tgt2
         (SIM: sim src0 tgt0)
         (STEP: Configuration.internal_step tgt0 tgt2),
@@ -91,7 +72,7 @@ Module Simulation.
         <<INTERNAL: Configuration.internal_steps src0 src1>> /\
         <<STEP: Configuration.internal_step src1 src2>> /\
         <<SIM: sim src2 tgt2>>
-    with internal_steps (B:BASE_STEP) (I:INCEPTION_STEP):
+    with internal_steps (B:BASE_STEP):
       forall src0 tgt0 tgt1
         (SIM: sim src0 tgt0)
         (STEP: Configuration.internal_steps tgt0 tgt1),
@@ -99,21 +80,21 @@ Module Simulation.
         <<INTERNAL: Configuration.internal_steps src0 src1>> /\
         <<SIM: sim src1 tgt1>>.
     Proof.
-      - i. inv STEP0.
-        + exploit B; eauto.
+      - i. inv STEP0; eapply B; eauto.
+        + congruence.
         + exploit internal_steps; eauto. i. des.
-          exploit I; eauto.
+          eexists _, _. splits; eauto.
       - i. revert src0 SIM. induction STEP0.
-        + i. exists src0. splits; eauto. econs.
+        + i. eexists. splits; eauto.
+          econs 1.
         + i. exploit internal_step; eauto. i. des.
           exploit IHSTEP0; eauto. i. des.
-          exists src3. splits; auto.
+          eexists. splits; [|eauto].
           eapply Configuration.internal_steps_append; eauto.
-          eapply Configuration.internal_steps_append; eauto.
-          econs; eauto. econs.
+          econs 2; eauto.
     Qed.
 
-    Lemma feasible_lemma (F:FEASIBLE) (B:BASE_STEP) (I:INCEPTION_STEP)
+    Lemma feasible_lemma (F:FEASIBLE) (B:BASE_STEP)
           src tgt
           (SIM: sim src tgt)
           (FEASIBLE: Configuration.feasible tgt):
@@ -125,7 +106,7 @@ Module Simulation.
       eapply Configuration.internal_steps_append; eauto.
     Qed.
 
-    Lemma step_lemma (F:FEASIBLE) (B:BASE_STEP) (I:INCEPTION_STEP) (E:EXTERNAL_STEP): STEP.
+    Lemma step_lemma (F:FEASIBLE) (B:BASE_STEP) (E:EXTERNAL_STEP): STEP.
     Proof.
       ii. inv STEP0.
       - exploit internal_step; eauto. i. des.
@@ -139,9 +120,8 @@ Module Simulation.
     Qed.
   End Simulation.
 
-  Structure t (prog_src prog_tgt:Program.syntax) := mk {
+  Structure t (prog_src prog_tgt:Configuration.syntax) := mk {
     sim: forall (src tgt:Configuration.t), Prop;
-
     init: INIT prog_src prog_tgt sim;
     step: STEP sim;
     terminal: TERMINAL sim;
